src/SeqExtra.v
@@ -9,7 +9,11 @@ Unset Printing Implicit Defensive.
 From Equations Require Import Equations.
 
 
-  Lemma filter_preserves_pred T (p pred : T -> bool) (s : seq T) :
+Section SeqExtra.
+
+  Variables (A B C : eqType) (T : Type).
+  
+  Lemma filter_preserves_pred (p pred : A -> bool) (s : seq A) :
     all p s ->
     all p [seq x <- s | pred x].
   Proof.
@@ -20,7 +24,7 @@ From Equations Require Import Equations.
       by apply: IH.
   Qed.
   
-  Lemma filter_all_predC1 (T : eqType) (s : seq T) (x : T) :
+  Lemma filter_all_predC1 (s : seq A) (x : A) :
     [seq x' <- s | predC1 x x'] = [::] ->
     forall x', x' \in s -> x' = x.
     elim: s x => [//| n s' IH] x /=.
@@ -30,13 +34,13 @@ From Equations Require Import Equations.
   Qed.
 
   
-  Lemma not_nil_spread {A : eqType} (lst : seq A) : lst != [::] -> exists x lst', lst = x :: lst'.
+  Lemma not_nil_spread (lst : seq A) : lst != [::] -> exists x lst', lst = x :: lst'.
   Proof.
       by case: lst => // x lst' H; exists x; exists lst'.  Qed.
 
   
 
-  Lemma ohead_in (A : eqType) (lst : seq A) (v : A) :
+  Lemma ohead_in (lst : seq A) (v : A) :
     ohead lst = Some v ->
     v \in lst.
   Proof.
@@ -46,14 +50,14 @@ From Equations Require Import Equations.
 
   
 
-  Lemma ohead_cons (A : eqType) H (x : A) lst :
+  Lemma ohead_cons H (x : A) lst :
     ohead (x :: lst) = H -> Some x = H.
   Proof. done. Qed.
 
 
   
 
-  Lemma map_fs {A B C : eqType} (lst : seq A) (f : A -> B -> C) (x y : B):
+  Lemma map_fs (lst : seq A) (f : A -> B -> C) (x y : B):
     (forall u,
       u \in lst ->
             f u x = f u y) ->
@@ -65,22 +69,66 @@ From Equations Require Import Equations.
     move/(_ (orTb (hd \in lst'))) => Hf. rewrite Hf.
     congr cons.
     move: H.
-  Admitted.
-
+  Abort.
   
 
-  Lemma singleton (A : Type) (x y : A) : x = y -> [:: x] = [:: y]. Proof. by move=> ->. Qed.
+  Lemma singleton (x y : A) : x = y -> [:: x] = [:: y]. Proof. by move=> ->. Qed.    
 
 
+  Fixpoint onth (s : seq T) (i : nat) : option T :=
+    match s, i with
+    | [::], _ => None
+    | (hd :: tl), 0 => Some hd
+    | (hd :: tl), n.+1 => onth tl n
+    end.
+
+
+
+ 
+  
+End SeqExtra.
+
+Section SeqI.
+  Variable (A : eqType).
+  
+  Definition seqI (s1 s2 : seq A) :=
+    undup (filter (mem s1) s2).
+  
+  Notation "s1 :&: s2" := (seqI s1 s2) : seq_scope.
+
+  Open Scope SEQ.
+
+  Lemma in_seqI (x : A) s1 s2 :
+    x \in (s1 :&: s2) = (x \in s1) && (x \in s2).
+  Proof.
+    by rewrite /seqI mem_undup mem_filter.
+  Qed.
+
+  Lemma seq1I (x : A) s1 :
+    [:: x] :&: s1 = if x \in s1 then [:: x] else [::].
+  Proof.
+    rewrite /seqI fun_if.
+    case: ifP => //= Hin; last first.
+  Admitted.
     
+  Lemma seq1I_N_nil (x : A) s1 :
+    [:: x] :&: s1 != [::] -> x \in s1.
+  Proof.
+    by rewrite seq1I; case: ifP.
+  Qed.
 
-
-    Fixpoint onth {T : Type} (s : seq T) (i : nat) : option T :=
-      match s, i with
-      | [::], _ => None
-      | (hd :: tl), 0 => Some hd
-      | (hd :: tl), n.+1 => onth tl n
-      end.
-
-
+  Lemma seq1IC x s1 :
+    [:: x] :&: s1 = s1 :&: [:: x].
+  Proof.
+    rewrite {2}/seqI /= seq1I.
+    by case: ifP.
+  Qed.
     
+End SeqI.
+
+Notation "s1 :&: s2" := (seqI s1 s2) : seq_scope.
+
+
+Arguments seqI [A].
+
+  
